scheduler/SchGInv.v
@@ -1,14 +1,12 @@
-Require Import CRIS.
+(* Require Import CRIS.
 
-Require Import SchInvariants.
+Require Import SchInvariants wpsim.
 
 Set Implicit Arguments.
 
 Section GINV.
-
   Context `{!invG α Σ Γ, !subHG Γ Σ, !sinvG Σ Γ α β τ}.
 
   Definition sch_ginv (univ: positive): Sk.t -> invspec :=
     fun _ _ => (∃ n, wsats univ n ⊤)%I.
-
-End GINV.
+End GINV. *)
