simulations/wpsim/wpsim_tactics.v
@@ -1,6 +1,0 @@
-Require Import Common.
-Require Import LAuto.
-
-Require Import Skeleton STB Mod SMod HMod PMod.
-Require Import wpsim.
-
