theories/simulations/wpsim/wpsim.v
@@ -1,0 +1,559 @@
+Require Import Common.
+
+Require Import ISim SMod SMod2HMod HMod.
+Require Import Skeleton.
+
+From stdpp Require Import coPset.
+
+Definition wpsim_ginv (u : univ_id) (n : level) (E : coPset)
+    `{!invG α Σ Γ, !subHG Γ Σ, !sinvG Σ Γ α β τ} : iProp Σ :=
+  own_admin ∗ univs u n ∗ wsats u n E.
+
+Class WP `{!invG α Σ Γ, !subHG Γ Σ, !sinvG Σ Γ α β τ} 
+    (P Q : iProp Σ) (υ : univ_id) (n : level) (E : coPset) :=
+  WP_iff : P ∗-∗ wpsim_ginv υ n E ∗ Q.
+
+Section wpsim.
+  Context `{!invG α Σ Γ, !subHG Γ Σ, !sinvG Σ Γ α β τ}.
+
+  Local Definition state : Type := alist key Any.t.
+  Local Definition post (R_s R_t : Type) : Type := nat → state * R_s → state * R_t → iProp Σ.
+  Local Definition rel : Type := ∀ R_s R_t : Type,
+    post R_s R_t → bool → bool → nat → state * itree hmodE R_s → state * itree hmodE R_t → iProp Σ.
+
+  Implicit Types r g : rel.
+  Implicit Types ps pt : bool.
+  Implicit Types nths : nat.
+  Implicit Types E : coPset.
+
+  (* TODO : abstraction into mixins *)
+  (* TODO : hard-code nodup conditions *)
+  (* Local Definition wpsim_pre u n E : iProp Σ := own_admin ∗ univs u n ∗ wsats u n E. *)
+  (* Local Definition wpsim_retcond υ n {R_s R_t} (RR : post R_s R_t) : post R_s R_t :=
+    (λ nths src tgt, RR nths src tgt ∗ wpsim_ginv υ n ⊤)%I. *)
+  Local Definition wpsim_rel υ n (r : rel) : rel :=
+    λ R_s R_t RR ps pt nths '(st_s, i_s) '(st_t, i_t),
+      (wpsim_ginv υ n ⊤ ∗ r R_s R_t RR ps pt nths (st_s, i_s) (st_t, i_t))%I.
+
+  (* Simulation relation that corresponds to iris' weakest precondition *)
+  Local Definition wpsim_def
+      fl_s fl_t Ist my_tid (t : option bool) υ ν n E r g R_s R_t RR ps pt nths st_s st_t
+      : iProp Σ :=
+  (* TODO : hide *)
+    (match t with
+    | None => emp
+    | Some false => wpsim_ginv ν n E -∗ wpsim_ginv υ n E
+    | Some true => wpsim_ginv υ n E
+    end) -∗
+    @isim Σ fl_s fl_t Ist my_tid false (wpsim_rel υ n r) (wpsim_rel υ n g)
+      R_s R_t RR ps pt nths st_s st_t.
+  Local Definition wpsim_aux : seal (@wpsim_def). Proof. by eexists. Qed.
+  Definition wpsim := wpsim_aux.(unseal).
+  Local Definition wpsim_eq : @wpsim = @wpsim_def := wpsim_aux.(seal_eq).
+  Local Ltac unseal := rewrite wpsim_eq /wpsim_def.
+
+  (* Variant wp_meta {X : nat → Type} : Type :=
+  | mk_wp_meta (n : nat) (x : X n).
+
+  Definition wp_fspec (υ : positive) (k : nat) (fsp : nat → fspec) : fspec :=
+    mk_fspec (meta := @wp_meta (λ n, (fsp n).(meta)))
+      (λ tid '(mk_wp_meta n x) varg arg,
+        wpsim_ginv υ (k + n) ⊤ ∗ (fsp n).(precond) tid x varg arg)%I
+      (λ tid '(mk_wp_meta n x) vret ret,
+        wpsim_ginv υ (k + n) ⊤ ∗ (fsp n).(postcond) tid x vret ret)%I. *)
+  Definition wp_fspec (υ : univ_id) (n : level) (fsp : fspec) : fspec :=
+    mk_fspec (meta := fsp.(meta))
+      (λ tid x varg arg,
+        wpsim_ginv υ n ⊤ ∗ fsp.(precond) tid x varg arg)%I
+      (λ tid x vret ret,
+        wpsim_ginv υ n ⊤ ∗ fsp.(postcond) tid x vret ret)%I.
+  
+  Global Instance wp_fspec_precond (fsp : fspec) (υ : univ_id) (n : level) tid m arg varg :
+    WP (precond (wp_fspec υ n fsp) tid m arg varg) (precond fsp tid m arg varg) υ n ⊤.
+  Proof. rewrite /precond /WP; ss; iSplit; iIntros "[$ $]". Qed.
+
+  Global Instance wp_fspec_postcond (fsp : fspec) (υ : univ_id) (n : level) tid m arg varg :
+    WP (postcond (wp_fspec υ n fsp) tid m arg varg) (postcond fsp tid m arg varg) υ n ⊤.
+  Proof. rewrite /postcond /WP; ss; iSplit; iIntros "[$ $]". Qed.
+
+  Section lemmas.
+    Context (fl_s fl_t : alist string (Any.t → itree hmodE Any.t)).
+    Context (Ist : nat → alist key Any.t → alist key Any.t → iProp Σ).
+    Context (my_tid : nat).
+    Context (t : option bool).
+    Context (υ ν : univ_id).
+    Context (n : level).
+    Context (R_s R_t : Type).
+    Context (RR : post R_s R_t).
+    Context (ps pt : bool).
+    Context (nths : nat).
+    Context (st_s st_t : state).
+  
+    (* Primitive simulation rules *)
+    Lemma wpsim_init sti_s sti_t :
+      (wpsim fl_s fl_t Ist my_tid (Some true) υ ν n ⊤ ibot ibot R_s R_t RR ps pt nths sti_s sti_t ∗
+      wpsim_ginv υ n ⊤) ⊢
+      @isim Σ fl_s fl_t Ist my_tid false ibot ibot R_s R_t RR ps pt nths sti_s sti_t.
+    Proof.
+      unseal; iIntros "[SIM I]"; iPoseProof ("SIM" with "I") as "SIM".
+      iPoseProof (isim_mono_knowledge with "SIM") as "SIM".
+      { instantiate (1:=ibot); i; iIntros "H"; rewrite /wpsim_rel /ibot; destruct sti_src, sti_tgt.
+        iDestruct "H" as "[_ []]".
+      }
+      { instantiate (1:=ibot); i; iIntros "H"; rewrite /wpsim_rel /ibot; destruct sti_src, sti_tgt.
+        iDestruct "H" as "[_ []]".
+      }
+      iFrame.
+    Qed.
+
+    (* Mostly will not be used *)
+    Lemma wpsim_ret r g rs rt :
+      RR nths (st_s, rs) (st_t, rt) ⊢
+      wpsim fl_s fl_t Ist my_tid t υ ν n ⊤ r g R_s R_t RR ps pt nths (st_s, Ret rs) (st_t, Ret rt).
+    Proof. unseal; iIntros "RR I". iApply isim_ret. iFrame. Qed.
+
+    Lemma wpsim_call r g E k_s k_t fn arg :
+      Ist nths st_s st_t ∗
+      (∀ ret nths' st_s' st_t'
+        (NODS : List.NoDup (List.map fst st_s'))
+        (NODD : List.NoDup (List.map fst st_t')),
+        Ist nths' st_s' st_t' -∗
+        wpsim fl_s fl_t Ist my_tid t υ ν n E r g R_s R_t RR true true nths'
+          (st_s', k_s ret) (st_t', k_t ret)) ⊢
+      wpsim fl_s fl_t Ist my_tid t υ ν n E r g R_s R_t RR ps pt nths
+        (st_s, trigger (Call fn arg) >>= k_s) (st_t, trigger (Call fn arg) >>= k_t).
+    Proof.
+      unseal; iIntros "[IST CONT] I".
+      rewrite -isim_call; iFrame.
+      iIntros (??????) "IST"; iApply ("CONT" with "[] [] [IST]"); iFrame; try iPureIntro; ss.
+    Qed.
+
+    Lemma wpsim_io r g fn I O (arg : I) k_s k_t E :
+      (∀ (ret : O),
+        wpsim fl_s fl_t Ist my_tid t υ ν n E r g R_s R_t RR true true nths
+          (st_s, k_s ret) (st_t, k_t ret)) ⊢
+      wpsim fl_s fl_t Ist my_tid t υ ν n E r g R_s R_t RR ps pt nths
+        (st_s, trigger (IO fn arg) >>= k_s)
+        (st_t, trigger (IO fn arg) >>= k_t).
+    Proof. unseal; iIntros "RR I". iApply isim_io. iIntros (ret); iApply "RR"; iFrame. Qed.
+
+    Lemma wpsim_tau_src r g i_s i_t E :
+      wpsim fl_s fl_t Ist my_tid t υ ν n E r g R_s R_t RR true pt nths (st_s, i_s) (st_t, i_t) ⊢
+      wpsim fl_s fl_t Ist my_tid t υ ν n E r g R_s R_t RR ps pt nths (st_s, tau;; i_s) (st_t, i_t).
+    Proof. unseal; iIntros "RR I". iApply isim_tau_src; iApply "RR"; iFrame. Qed.
+
+    Lemma wpsim_tau_tgt r g i_s i_t E :
+      wpsim fl_s fl_t Ist my_tid t υ ν n E r g R_s R_t RR ps true nths (st_s, i_s) (st_t, i_t) ⊢
+      wpsim fl_s fl_t Ist my_tid t υ ν n E r g R_s R_t RR ps pt nths (st_s, i_s) (st_t, tau;; i_t).
+    Proof. unseal; iIntros "RR I". iApply isim_tau_tgt; iApply "RR"; iFrame. Qed.
+
+    Lemma wpsim_inline_src r g fn arg f_s k_s i_t E :
+      alist_find fn fl_s = Some f_s →
+      wpsim fl_s fl_t Ist my_tid t υ ν n E r g R_s R_t RR true pt nths
+        (st_s, x <- (ret <- (f_s arg);; (tau;; tau;; Ret ret));; (k_s x))
+        (st_t, i_t) ⊢
+      wpsim fl_s fl_t Ist my_tid t υ ν n E r g R_s R_t RR ps pt nths
+        (st_s, trigger (Call fn arg) >>= k_s) (st_t, i_t).
+    Proof. i; unseal; iIntros "RR I". iApply isim_inline_src; eauto. iApply "RR"; iFrame. Qed.
+
+    Lemma wpsim_inline_tgt r g fn arg i_s f_t k_t E :
+      alist_find fn fl_t = Some f_t →
+      wpsim fl_s fl_t Ist my_tid t υ ν n E r g R_s R_t RR ps true nths
+        (st_s, i_s)
+        (st_t, x <- (ret <- (f_t arg);; (tau;; tau;; Ret ret));; (k_t x)) ⊢
+      wpsim fl_s fl_t Ist my_tid t υ ν n E r g R_s R_t RR ps pt nths
+        (st_s, i_s) (st_t, trigger (Call fn arg) >>= k_t).
+    Proof. i; unseal; iIntros "RR I". iApply isim_inline_tgt; eauto. iApply "RR"; iFrame. Qed.
+
+    Lemma wpsim_take_src X r g k_s i_t E :
+      (∀ x, wpsim fl_s fl_t Ist my_tid t υ ν n E r g R_s R_t RR true pt nths
+        (st_s, k_s x) (st_t, i_t)) ⊢
+      wpsim fl_s fl_t Ist my_tid t υ ν n E r g R_s R_t RR ps pt nths
+        (st_s, trigger (Take X) >>= k_s) (st_t, i_t).
+    Proof.
+      unseal; iIntros "RR I". iApply isim_take_src; eauto. iIntros (x); iApply "RR"; iFrame.
+    Qed.
+
+    Lemma wpsim_take_tgt X r g i_s k_t E :
+      (∃ x,
+        wpsim fl_s fl_t Ist my_tid t υ ν n E r g R_s R_t RR ps true nths (st_s, i_s) (st_t, k_t x)) ⊢
+      wpsim fl_s fl_t Ist my_tid t υ ν n E r g R_s R_t RR ps pt nths
+        (st_s, i_s) (st_t, trigger (Take X) >>= k_t).
+    Proof.
+      unseal; iIntros "[%x RR] I". iApply isim_take_tgt; eauto. iExists _; iApply "RR"; iFrame.
+    Qed.
+
+    Lemma wpsim_choose_src X r g k_s i_t E :
+      (∃ x,
+        wpsim fl_s fl_t Ist my_tid t υ ν n E r g R_s R_t RR true pt nths (st_s, k_s x) (st_t, i_t)) ⊢
+      wpsim fl_s fl_t Ist my_tid t υ ν n E r g R_s R_t RR ps pt nths
+        (st_s, trigger (Choose X) >>= k_s) (st_t, i_t).
+    Proof.
+      unseal; iIntros "[%x RR] I". iApply isim_choose_src; eauto. iExists _; iApply "RR"; iFrame.
+    Qed.
+
+    Lemma wpsim_choose_tgt X r g i_s k_t E :
+      (∀ x,
+        wpsim fl_s fl_t Ist my_tid t υ ν n E r g R_s R_t RR ps true nths (st_s, i_s) (st_t, k_t x)) ⊢
+      wpsim fl_s fl_t Ist my_tid t υ ν n E r g R_s R_t RR ps pt nths
+        (st_s, i_s) (st_t, trigger (Choose X) >>= k_t).
+    Proof.
+      unseal; iIntros "RR I". iApply isim_choose_tgt; eauto. iIntros (x); iApply "RR"; iFrame.
+    Qed.
+
+    Lemma wpsim_sput_src k v r g k_s i_t E :
+      wpsim fl_s fl_t Ist my_tid t υ ν n E r g R_s R_t RR true pt nths
+        (alist_upd k v st_s, k_s tt) (st_t, i_t) ⊢
+      wpsim fl_s fl_t Ist my_tid t υ ν n E r g R_s R_t RR ps pt nths
+        (st_s, trigger (SPut k v) >>= k_s) (st_t, i_t).
+    Proof. unseal; iIntros "RR I". iApply isim_sput_src; eauto. iApply "RR"; iFrame. Qed.
+
+    Lemma wpsim_sput_tgt k v r g i_s k_t E :
+      wpsim fl_s fl_t Ist my_tid t υ ν n E r g R_s R_t RR ps true nths
+        (st_s, i_s) (alist_upd k v st_t, k_t tt) ⊢
+      wpsim fl_s fl_t Ist my_tid t υ ν n E r g R_s R_t RR ps pt nths
+        (st_s, i_s) (st_t, trigger (SPut k v) >>= k_t).
+    Proof. unseal; iIntros "RR I". iApply isim_sput_tgt; eauto. iApply "RR"; iFrame. Qed.
+
+    Lemma wpsim_sget_src k r g k_s i_t E :
+      wpsim fl_s fl_t Ist my_tid t υ ν n E r g R_s R_t RR true pt nths
+        (st_s, k_s (or_else (alist_find k st_s) tt↑)) (st_t, i_t) ⊢
+      wpsim fl_s fl_t Ist my_tid t υ ν n E r g R_s R_t RR ps pt nths
+        (st_s, trigger (SGet k) >>= k_s) (st_t, i_t).
+    Proof. unseal; iIntros "RR I". iApply isim_sget_src; eauto. iApply "RR"; iFrame. Qed.
+
+    Lemma wpsim_sget_tgt k r g i_s k_t E :
+      wpsim fl_s fl_t Ist my_tid t υ ν n E r g R_s R_t RR ps true nths
+        (st_s, i_s) (st_t, k_t (or_else (alist_find k st_t) tt↑)) ⊢
+      wpsim fl_s fl_t Ist my_tid t υ ν n E r g R_s R_t RR ps pt nths
+        (st_s, i_s) (st_t, trigger (SGet k) >>= k_t).
+    Proof. unseal; iIntros "RR I". iApply isim_sget_tgt; eauto. iApply "RR"; iFrame. Qed.
+
+    Lemma wpsim_assume_src (P : iProp Σ) r g k_s i_t E :
+      (P -∗ wpsim fl_s fl_t Ist my_tid t υ ν n E r g R_s R_t RR true pt nths
+        (st_s, k_s tt) (st_t, i_t)) ⊢
+      wpsim fl_s fl_t Ist my_tid t υ ν n E r g R_s R_t RR ps pt nths
+        (st_s, trigger (Assume P) >>= k_s) (st_t, i_t).
+    Proof.
+      unseal; iIntros "RR I". iApply isim_Assume_src; eauto. iIntros "P".
+      iApply ("RR" with "P"); iFrame.
+    Qed.
+
+    Lemma wpsim_assume_tgt (P : iProp Σ) r g i_s k_t E :
+      P ∗ wpsim fl_s fl_t Ist my_tid t υ ν n E r g R_s R_t RR ps true nths
+        (st_s, i_s) (st_t, k_t tt) ⊢
+      wpsim fl_s fl_t Ist my_tid t υ ν n E r g R_s R_t RR ps pt nths
+        (st_s, i_s) (st_t, trigger (Assume P) >>= k_t).
+    Proof. unseal; iIntros "[P RR] I". iApply isim_Assume_tgt; eauto. iFrame. iApply "RR". ss. Qed.
+
+    Lemma wpsim_guarantee_src (P : iProp Σ) r g k_s i_t E :
+      P ∗ wpsim fl_s fl_t Ist my_tid t υ ν n E r g R_s R_t RR true pt nths
+        (st_s, k_s tt) (st_t, i_t) ⊢
+      wpsim fl_s fl_t Ist my_tid t υ ν n E r g R_s R_t RR ps pt nths
+        (st_s, trigger (Guarantee P) >>= k_s) (st_t, i_t).
+    Proof.
+      unseal; iIntros "[P RR] I". iApply isim_Guarantee_src; eauto. iFrame. iApply "RR"; ss.
+    Qed.
+
+    Lemma wpsim_guarantee_tgt (P : iProp Σ) r g i_s k_t E :
+      P ∗ wpsim fl_s fl_t Ist my_tid t υ ν n E r g R_s R_t RR ps true nths
+        (st_s, i_s) (st_t, k_t tt) ⊢
+      wpsim fl_s fl_t Ist my_tid t υ ν n E r g R_s R_t RR ps pt nths
+        (st_s, i_s) (st_t, trigger (Assume P) >>= k_t).
+    Proof. unseal; iIntros "[P RR] I". iApply isim_Assume_tgt; eauto. iFrame. iApply "RR". ss. Qed.
+
+    Lemma wpsim_spawn r g fn args k_s k_t E :
+      wpsim fl_s fl_t Ist my_tid t υ ν n E r g R_s R_t RR true true (S nths)
+        (st_s, k_s nths) (st_t, k_t nths) ⊢
+      wpsim fl_s fl_t Ist my_tid t υ ν n E r g R_s R_t RR ps pt nths
+        (st_s, trigger (Spawn fn args) >>= k_s)
+        (st_t, trigger (Spawn fn args) >>= k_t).
+    Proof. unseal; iIntros "C I". iApply isim_spawn; eauto. iApply "C". ss. Qed.
+
+    Lemma wpsim_yield r g tid k_s k_t E :
+      Ist nths st_s st_t ∗
+      (∀ nths' st_s' st_t' (NODS : List.NoDup (map fst st_s')) (NODT : List.NoDup (map fst st_t')),
+        Ist nths' st_s' st_t' -∗
+        wpsim fl_s fl_t Ist my_tid t υ ν n E r g R_s R_t RR true true nths'
+          (st_s', k_s tt) (st_t', k_t tt)) ⊢
+      wpsim fl_s fl_t Ist my_tid t υ ν n E r g R_s R_t RR ps pt nths
+        (st_s, trigger (Yield tid) >>= k_s)
+        (st_t, trigger (Yield tid) >>= k_t).
+    Proof.
+      unseal; iIntros "[IST C] I". iApply isim_yield; eauto. iFrame.
+      iIntros (?????) "IST"; iApply ("C" with "[] [] [IST] [I]"); iFrame; iPureIntro; ss.
+    Qed.
+
+    Lemma wpsim_tid_src r g k_s i_t E :
+      wpsim fl_s fl_t Ist my_tid t υ ν n E r g R_s R_t RR true pt nths
+        (st_s, k_s my_tid) (st_t, i_t) ⊢
+      wpsim fl_s fl_t Ist my_tid t υ ν n E r g R_s R_t RR ps pt nths
+        (st_s, trigger Tid >>= k_s) (st_t, i_t).
+    Proof. unseal; iIntros "RR I". iApply isim_tid_src; iApply "RR"; iFrame. Qed.
+
+    Lemma wpsim_tid_tgt r g i_s k_t E :
+      wpsim fl_s fl_t Ist my_tid t υ ν n E r g R_s R_t RR ps true nths
+        (st_s, i_s) (st_t, k_t my_tid) ⊢
+      wpsim fl_s fl_t Ist my_tid t υ ν n E r g R_s R_t RR ps pt nths
+        (st_s, i_s) (st_t, trigger Tid >>= k_t).
+    Proof. unseal; iIntros "RR I". iApply isim_tid_tgt; iApply "RR"; iFrame. Qed.
+
+    Lemma wpsim_reset r g i_s i_t E :
+      wpsim fl_s fl_t Ist my_tid t υ ν n E r g R_s R_t RR false false nths (st_s, i_s) (st_t, i_t) ⊢
+      wpsim fl_s fl_t Ist my_tid t υ ν n E r g R_s R_t RR ps pt nths (st_s, i_s) (st_t, i_t).
+    Proof. unseal; iIntros "RR I". iApply isim_reset; iApply "RR"; iFrame. Qed.
+
+    Lemma wpsim_progress r g i_s i_t E :
+      wpsim fl_s fl_t Ist my_tid t υ ν n E g g R_s R_t RR false false nths (st_s, i_s) (st_t, i_t) ⊢
+      wpsim fl_s fl_t Ist my_tid t υ ν n E r g R_s R_t RR true true nths (st_s, i_s) (st_t, i_t).
+    Proof. unseal; iIntros "RR I". iApply isim_progress; iApply "RR"; iFrame. Qed.
+
+    Lemma wpsim_base r g i_s i_t :
+      r R_s R_t RR ps pt nths (st_s, i_s) (st_t, i_t) ⊢
+      wpsim fl_s fl_t Ist my_tid (Some true) υ ν n ⊤ r g R_s R_t RR ps pt nths
+        (st_s, i_s) (st_t, i_t).
+    Proof. unseal; iIntros "RR I". iApply isim_base; iFrame. Qed.
+
+    Lemma wpsim_coind (r g : rel) A P RA_s RA_t RRA psA ptA nthsA srcA tgtA :
+      (∀ (g' : rel) (a : A),
+        P a -∗
+        (□ ∀ R_s R_t RR ps pt nths0 src tgt,
+          g R_s R_t RR ps pt nths0 src tgt -∗ g' R_s R_t RR ps pt nths0 src tgt) -∗
+        (□ ∀ a, P a -∗ g' (RA_s a) (RA_t a) (RRA a) (psA a) (ptA a) (nthsA a) (srcA a) (tgtA a)) -∗
+        wpsim fl_s fl_t Ist my_tid (Some true) υ ν n ⊤ r g'
+          (RA_s a) (RA_t a) (RRA a) (psA a) (ptA a) (nthsA a) (srcA a) (tgtA a)) →
+      ∀ (a : A), P a ⊢
+        wpsim fl_s fl_t Ist my_tid (Some true) υ ν n ⊤ r g
+          (RA_s a) (RA_t a) (RRA a) (psA a) (ptA a) (nthsA a) (srcA a) (tgtA a).
+    Proof.
+      unseal; intros H a; iIntros "P I"; iCombine "P I" as "P". iStopProof.
+      (* rewrite /wpsim_retcond *)
+      revert a. eapply isim_coind.
+      intros g' a Himpl; iIntros "[[P I] #CIH]".
+      iPoseProof (H with "P [] [] I") as "H".
+      { instantiate (1 :=
+          (λ R_s R_t RR ps pt nths '(st_s, i_s) '(st_t, i_t),
+            wpsim_ginv υ n ⊤ -∗
+            g' R_s R_t RR ps pt nths (st_s, i_s) (st_t, i_t))%I).
+        iModIntro; iIntros (????????) "G"; destruct src, tgt; iIntros "I". iApply Himpl. iFrame.
+      }
+      { iModIntro; iIntros (a') "P"; iSpecialize ("CIH" $! a'); destruct (srcA a'), (tgtA a').
+        iIntros "I"; iApply "CIH"; iFrame.
+      }
+      iApply (isim_mono_knowledge with "H"); ss.
+      { iIntros (????????) "H"; iModIntro; iFrame. }
+      { iIntros (????????) "H !>"; destruct sti_src, sti_tgt; rewrite /wpsim_rel.
+        iDestruct "H" as "[H1 H2]"; iApply "H2"; iFrame.
+      }
+    Qed.
+
+    (* ginv related lemmas *)
+    Lemma wpsim_full_guarantee_src_WP `{!WP P Q υ n E} r g k_s i_t :
+      (Q ∗
+      wpsim fl_s fl_t Ist my_tid None υ ν n E r g R_s R_t RR true pt nths
+        (st_s, k_s tt) (st_t, i_t)) ⊢
+      wpsim fl_s fl_t Ist my_tid (Some true) υ ν n E r g R_s R_t RR ps pt nths
+        (st_s, trigger (Guarantee P) >>= k_s) (st_t, i_t).
+    Proof.
+      unseal; iIntros "[P SIM] I". iApply isim_Guarantee_src; eauto.
+      iSplitR "SIM".
+      { iApply WP_iff; iFrame. }
+      { iApply "SIM"; done. }
+    Qed.
+
+    Lemma wpsim_full_guarantee_src (P : iProp Σ) r g k_s i_t E :
+      ((wpsim_ginv υ n E -∗ P) ∗
+      wpsim fl_s fl_t Ist my_tid None υ ν n E r g R_s R_t RR true pt nths
+        (st_s, k_s tt) (st_t, i_t)) ⊢
+      wpsim fl_s fl_t Ist my_tid (Some true) υ ν n E r g R_s R_t RR ps pt nths
+        (st_s, trigger (Guarantee P) >>= k_s) (st_t, i_t).
+    Proof.
+      unseal; iIntros "[P SIM] I". iApply isim_Guarantee_src; eauto.
+      iSplitR "SIM"; iFrame. iApply "P"; iFrame. iApply "SIM"; done.
+    Qed.
+
+    Lemma wpsim_full_assume_src (P P' : iProp Σ) r g k_s i_t E :
+      ((P -∗ (wpsim_ginv υ n E ∗ P')) ∗
+      (P' -∗ wpsim fl_s fl_t Ist my_tid (Some true) υ ν n E r g R_s R_t RR true pt nths
+        (st_s, k_s tt) (st_t, i_t))) ⊢
+      wpsim fl_s fl_t Ist my_tid None υ ν n E r g R_s R_t RR ps pt nths
+        (st_s, trigger (Assume P) >>= k_s) (st_t, i_t).
+    Proof.
+      unseal; iIntros "[P SIM] I". iApply isim_Assume_src; eauto.
+      iIntros "P'". iPoseProof ("P" with "P'") as "[GINV P]".
+      iApply ("SIM" with "P GINV").
+    Qed.
+
+    Lemma wpsim_full_assume_src_WP `{!WP P Q υ n E} r g k_s i_t :
+      (Q -∗ wpsim fl_s fl_t Ist my_tid (Some true) υ ν n E r g R_s R_t RR true pt nths
+        (st_s, k_s tt) (st_t, i_t)) ⊢
+      wpsim fl_s fl_t Ist my_tid None υ ν n E r g R_s R_t RR ps pt nths
+        (st_s, trigger (Assume P) >>= k_s) (st_t, i_t).
+    Proof.
+      unseal; iIntros "SIM _". iApply isim_Assume_src; eauto.
+      iIntros "P". iPoseProof (WP_iff with "P") as "[I Q]".
+      iApply ("SIM" with "Q I").
+    Qed.
+
+    (* Derived lemmas *)
+    Lemma wpsim_unwrapN_src r g X (x : option X) k_s i_t E :
+      (∃ x', ⌜x = Some x'⌝ ∗
+        wpsim fl_s fl_t Ist my_tid t υ ν n E r g R_s R_t RR ps pt nths
+          (st_s, k_s x') (st_t, i_t)) ⊢
+      wpsim fl_s fl_t Ist my_tid t υ ν n E r g R_s R_t RR ps pt nths
+        (st_s, unwrapN x >>= k_s) (st_t, i_t).
+    Proof. iIntros "H". iDestruct "H" as (x') "[% H]". subst. hred_l. iApply "H". Qed.
+
+    Lemma wpsim_sput_src_sandbox scopes k v r g k_s i_t E :
+      In k.1 scopes →
+      wpsim fl_s fl_t Ist my_tid t υ ν n E r g R_s R_t RR true pt nths
+        (alist_upd k v st_s, k_s tt) (st_t, i_t) ⊢
+      wpsim fl_s fl_t Ist my_tid t υ ν n E r g R_s R_t RR ps pt nths
+        (st_s, HModSem.sandbox scopes (trigger (SPut k v)) >>= k_s) (st_t, i_t).
+    Proof.
+      intros IN; iIntros "SIM".
+      rewrite HModSB.transl_put; des_ifs; ss.
+      { iApply wpsim_sput_src; ss. }
+      { edestruct (existsb_exists (String.eqb k.1) scopes).
+        hexploit H0; ss.
+        { exists k.1; split; ss. apply String.eqb_refl. }
+        { i; clarify. }
+      }
+    Qed.
+
+    Lemma wpsim_sget_src_sandbox scopes k r g k_s i_t E :
+      In k.1 scopes →
+      wpsim fl_s fl_t Ist my_tid t υ ν n E r g R_s R_t RR true pt nths
+        (st_s, k_s (or_else (alist_find k st_s) tt↑)) (st_t, i_t) ⊢
+      wpsim fl_s fl_t Ist my_tid t υ ν n E r g R_s R_t RR ps pt nths
+        (st_s, HModSem.sandbox scopes (trigger (SGet k)) >>= k_s) (st_t, i_t).
+    Proof.
+      intros IN; iIntros "SIM".
+      rewrite HModSB.transl_get; des_ifs; ss.
+      { iApply wpsim_sget_src; ss. }
+      { edestruct (existsb_exists (String.eqb k.1) scopes).
+        hexploit H0; ss.
+        { exists k.1; split; ss. apply String.eqb_refl. }
+        { i; clarify. }
+      }
+    Qed.
+
+    Lemma wpsim_sput_tgt_sandbox scopes k v r g i_s k_t E :
+      In k.1 scopes →
+      wpsim fl_s fl_t Ist my_tid t υ ν n E r g R_s R_t RR ps true nths
+        (st_s, i_s) (alist_upd k v st_t, k_t tt) ⊢
+      wpsim fl_s fl_t Ist my_tid t υ ν n E r g R_s R_t RR ps pt nths
+        (st_s, i_s) (st_t, HModSem.sandbox scopes (trigger (SPut k v)) >>= k_t).
+    Proof.
+      intros IN; iIntros "SIM".
+      rewrite HModSB.transl_put; des_ifs; ss.
+      { iApply wpsim_sput_tgt; ss. }
+      { edestruct (existsb_exists (String.eqb k.1) scopes).
+        hexploit H0; ss.
+        { exists k.1; split; ss. apply String.eqb_refl. }
+        { i; clarify. }
+      }
+    Qed.
+
+    Lemma wpsim_sget_tgt_sandbox scopes k r g i_s k_t E :
+      In k.1 scopes →
+      wpsim fl_s fl_t Ist my_tid t υ ν n E r g R_s R_t RR ps true nths
+        (st_s, i_s) (st_t, k_t (or_else (alist_find k st_t) tt↑)) ⊢
+      wpsim fl_s fl_t Ist my_tid t υ ν n E r g R_s R_t RR ps pt nths
+        (st_s, i_s) (st_t, HModSem.sandbox scopes (trigger (SGet k)) >>= k_t).
+    Proof.
+      intros IN; iIntros "SIM".
+      rewrite HModSB.transl_get; des_ifs; ss.
+      { iApply wpsim_sget_tgt; ss. }
+      { edestruct (existsb_exists (String.eqb k.1) scopes).
+        hexploit H0; ss.
+        { exists k.1; split; ss. apply String.eqb_refl. }
+        { i; clarify. }
+      }
+    Qed.
+
+    Lemma wpsim_asm_src (P : Prop) r g k_s i_t E :
+      (∀ _ : P, (wpsim fl_s fl_t Ist my_tid t υ ν n E r g R_s R_t RR true pt nths
+        (st_s, k_s tt) (st_t, i_t))) ⊢
+      wpsim fl_s fl_t Ist my_tid t υ ν n E r g R_s R_t RR ps pt nths
+        (st_s, assume P >>= k_s) (st_t, i_t).
+    Proof.
+      unseal; iIntros "RR I". iApply isim_asm_src; eauto.
+      iIntros "%H"; iApply ("RR" $! H with "I"); iFrame.
+    Qed.
+
+    Lemma wpsim_asm_tgt (P : Prop) r g i_s k_t E :
+      P →
+      wpsim fl_s fl_t Ist my_tid t υ ν n E r g R_s R_t RR ps true nths
+        (st_s, i_s) (st_t, k_t tt) ⊢
+      wpsim fl_s fl_t Ist my_tid t υ ν n E r g R_s R_t RR ps pt nths
+        (st_s, i_s) (st_t, assume P >>= k_t).
+    Proof.
+      intros H; unseal; iIntros "P I". iApply isim_asm_tgt; eauto. iApply ("P" with "I").
+    Qed.
+
+    Lemma wpsim_guar_src (P : Prop) r g k_s i_t E :
+      P →
+      wpsim fl_s fl_t Ist my_tid t υ ν n E r g R_s R_t RR true pt nths
+        (st_s, k_s tt) (st_t, i_t) ⊢
+      wpsim fl_s fl_t Ist my_tid t υ ν n E r g R_s R_t RR ps pt nths
+        (st_s, guarantee P >>= k_s) (st_t, i_t).
+    Proof.
+      intros H; unseal; iIntros "P I". iApply isim_guar_src; eauto. iApply ("P" with "I").
+    Qed.
+
+    Lemma wpsim_guar_tgt (P : Prop) r g i_s k_t E :
+      (∀ _ : P, wpsim fl_s fl_t Ist my_tid t υ ν n E r g R_s R_t RR ps true nths
+        (st_s, i_s) (st_t, k_t tt)) ⊢
+      wpsim fl_s fl_t Ist my_tid t υ ν n E r g R_s R_t RR ps pt nths
+        (st_s, i_s) (st_t, guarantee P >>= k_t).
+    Proof.
+      unseal; iIntros "RR I". iApply isim_guar_tgt; eauto.
+      iIntros "%H"; iApply ("RR" $! H with "I"); iFrame.
+    Qed.
+
+    (* Proofmode instances *)
+    Global Instance wpsim_elim_upd r g P p i_s i_t E :
+      ElimModal True p false ( |==> P)%I P
+        (wpsim fl_s fl_t Ist my_tid t υ ν n E r g R_s R_t RR ps pt nths (st_s, i_s) (st_t, i_t))
+        (wpsim fl_s fl_t Ist my_tid t υ ν n E r g R_s R_t RR ps pt nths (st_s, i_s) (st_t, i_t)).
+    Proof.
+      unseal.
+      unfold ElimModal. rewrite bi.intuitionistically_if_elim.
+      i. iIntros "[H0 H1] HPRE".
+      iApply isim_upd. iMod "H0". iModIntro.
+      iApply ("H1" with "H0 HPRE").
+    Qed.
+End lemmas. End wpsim.
+
+(* Section test. *)
+  (* Context `{!invG α Σ Γ, !subHG Γ Σ, !sinvG Σ Γ α β τ}. *)
+  (* Context (m_s : SMod.t). *)
+  (* Context (m_t : HMod.t). *)
+  (* Context (ginv : Sk.t → nat → iProp Σ). *)
+  (* Context (stb : Sk.t → gname → option fspec). *)
+  (* Context (body_s body_t : Any.t → itree hmodE Any.t). *)
+  (* Context (fl_s fl_t : alist string (Any.t → itree hmodE Any.t)). *)
+  (* Context (my_tid : nat). *)
+  (* Context (u : univ_id). *)
+  (* Context (k : level). *)
+  (* Context (spec_s : nat → fspec). *)
+
+  (* Context (init_cond : Sk.t → iProp Σ). *)
+  (* Context (Ist : Sk.t → nat → alist key Any.t → alist key Any.t → iProp Σ). *)
+  (* Goal ∀ sk nths st_s st_t RR arg, *)
+    (* (∀ n, *)
+      (* Ist sk nths st_s st_t ⊢ *)
+      (* @wpsim α Σ Γ _ _  β fl_s fl_t (Ist sk) my_tid u n ibot ibot Any.t RR false false nths *)
+        (* (st_s, interp_sb_hp (ginv sk) (stb sk) (mk_specbody (spec_s (k + n)) body_s) arg) *)
+        (* (st_t, body_t arg) ⊤) → *)
+    (* (Ist sk nths st_s st_t ⊢ *)
+    (* @isim Σ fl_s fl_t (Ist sk) my_tid false ibot ibot Any.t RR false false nths *)
+      (* (st_s, interp_sb_hp (ginv sk) (stb sk) (mk_specbody (wp_fspec u k spec_s) body_s) arg) *)
+      (* (st_t, body_t arg)). *)
+  (* Proof. *)
+    (* rewrite /interp_sb_hp /HoareFun; ss. *)
+    (* ii. iIntros "IST". step_l. *)
+  (* Admitted. *)
+(* End test. *)
+(* TODO : proofmode instances *)
